prove lemma_QuorumIntersection

paxos/proof_helper.dfy
@@ -48,16 +48,67 @@ lemma Lemma_DecidedImpliesQuorumOfAccepts(c:Constants, ds:DistrSys, idx:int)
 
 
 
-lemma lemma_QuorumIntersection(c:Constants, ds:DistrSys, p1_qrm:set<Packet>, p1_bal:Ballot, p2_qrm:set<Packet>, p2_bal:Ballot)
+lemma {:timeLimitMultiplier 2} lemma_QuorumIntersection(c:Constants, ds:DistrSys, p1_qrm:set<Packet>, p1_bal:Ballot, p2_qrm:set<Packet>, p2_bal:Ballot)
+returns (acc_id:Id)
     requires c.WF() && ds.WF(c)
     requires AllPacketsValid(c, ds)
     requires QuorumOfPromiseMsgs(c, ds, p1_qrm, p1_bal)
     requires QuorumOfAcceptMsgs(c, ds, p2_qrm, p2_bal)
-    ensures exists acc_id :: 
-                    && (exists prom_p : Packet :: prom_p in p1_qrm && prom_p.src == acc_id)
-                    && (exists acc_p : Packet :: acc_p in p2_qrm && acc_p.src == acc_id)
+    ensures acc_id.agt == Acc && c.ValidAccIdx(acc_id.idx)
+    ensures && (exists prom_p : Packet :: prom_p in p1_qrm && prom_p.src == acc_id)
+            && (exists acc_p : Packet :: acc_p in p2_qrm && acc_p.src == acc_id)
 {
-    assume false;  
+    var p1_src_qrm := extractPacketSources(p1_qrm);
+    var p2_src_qrm := extractPacketSources(p2_qrm);
+    assert forall id | id in p1_src_qrm :: id in c.acc_ids;
+    assert forall id | id in p2_src_qrm :: id in c.acc_ids;
+
+    if forall id | id in c.acc_ids :: !(id in p1_src_qrm && id in p2_src_qrm) {
+        assert seqIsUnique(c.acc_ids);
+        var acc_ids := setFromSeq(c.acc_ids);
+        assert |acc_ids| == 2*c.f+1;
+        var e := lemma_Set_Intersection(p1_src_qrm, p2_src_qrm, acc_ids);
+        assert e in acc_ids && e in p1_src_qrm && e in p2_src_qrm;
+        assert false;
+    }
+    acc_id :| acc_id in c.acc_ids && acc_id in p1_src_qrm && acc_id in p2_src_qrm;
+}
+
+
+function extractPacketSources(S:set<Packet>) : (res:set<Id>) 
+    decreases S
+    ensures forall id | id in res :: (exists p :: p in S && p.src == id)
+    ensures forall p | p in S :: p.src in res
+    ensures UniqueSources(S) ==> |res| == |S|
+{ 
+    if |S| == 0 then {}
+    else 
+        var p :| p in S;
+        {p.src} + extractPacketSources(S - {p})
+}
+
+
+function setFromSeq(a:seq<Id>) : (res:set<Id>) 
+    decreases a
+    ensures forall i | 0 <= i < |a| :: a[i] in res
+    ensures forall id | id in res :: (exists i :: 0 <= i < |a| && a[i] == id)
+    ensures seqIsUnique(a) ==> |a| == |res|
+{ 
+    if |a| == 0 then {}
+    else 
+        {a[0]} + setFromSeq(a[1..])
+}
+
+
+lemma lemma_Set_Intersection(S1:set<Id>, S2:set<Id>, U:set<Id>) returns (e:Id)
+    requires |S1| > |U|/2
+    requires |S2| > |U|/2
+    requires forall id | id in S1 :: id in U
+    requires forall id | id in S2 :: id in U
+    ensures e in U && e in S1 && e in S2
+{
+    // TODO: assume for now
+    assume false;
 }
 
 }
