paxos/types.dfy
@@ -47,5 +47,9 @@ function {:opaque} NextBallot(b:Ballot, idx:nat) : (b':Ballot)
     else Ballot(b.seqNo + 1, idx)
 }
 
+predicate seqIsUnique<T>(a:seq<T>) {
+    forall i, j | 0<=i<|a| && 0<=j<|a| && a[i]==a[j] :: i == j
+}
+
 
 }
